[sledge sem] Start sketching translation correctness
Summary:
This includes a few changes and corrections to the semantics, to support
the translation. This initial attempt to reason about LLVM -> llair
showed three things that needed repair in the semantics, in addition to
various bugs. We address them as follows.

Refactor llair semantics to have only a single kind of flat value:
integers that fit into specified bit widths. Operations on size values
(e.g., offsets, indices and the like) can just take an integer and
ignore its number of bits. Pointers can just be considered integers that
fit into a certain size given by the constant pointer_size. Later on we
can consider making this a parameter to the model.

Change the generic memory model interface to use numbers rather than
words as the generic encoding of a large value. This makes it more
useful for llair where words are not used.

Pay more careful attention to signed/unsigned issues. Neither LLVM nor
llair have a concept of signed vs unsigned value. Instead individual
operations interpret bit patterns in various ways, some of which are
ambiguous in the LLVM manual. For example, since getelementpointer's
indices are explicitly said to be interpreted as signed 2's complement,
we should probably do the same for insertvalue and extractvalue. However
it is not clear how the argument to alloca is to be interpreted. For now
we assume signed.

Reviewed By: jberdine

Differential Revision: D17164133

fbshipit-source-id: 31a8af635

sledge/semantics/llairScript.sml
@@ -19,6 +19,7 @@ numLib.prefer_num ();
 Datatype:
   typ =
   | FunctionT typ (typ list)
+  (* How many bits the integer occupies *)
   | IntegerT num
   | PointerT typ
   | ArrayT typ num
@@ -121,13 +122,11 @@ End
 (* ----- Semantic states ----- *)
 
 (* These are the values that can be stored in registers. The implementation uses
- * integers with a bit-width to represent numbers, and keeps locations and sizes
- * separate.
+ * integers with a bit-width to represent numbers and pointers. Here we
+ * interpret the bit width b as meaning the int should be in the range [-2^(b-1),2^(b-1))
  *)
 Datatype:
   flat_v =
-  | LocV num
-  | SizeV num
   | IntV int num
 End
 
@@ -143,32 +142,26 @@ Datatype:
        globals : var |-> word64;
        locals : var |-> v;
        stack : frame list;
-       pointer_size : 'a itself;
        heap : unit heap |>
+End
+
+(* Assume that all pointers can fit in 64 bits *)
+Definition pointer_size_def:
+  pointer_size = 64
 End
 
 (* ----- Semantic transitions ----- *)
 
+(* The size of a type in bytes, rounded up *)
 Definition sizeof_def:
-  (sizeof (:'a) (IntegerT n) = n) ∧
-  (sizeof (:'a) (PointerT t) = dimindex (:'a)) ∧
-  (sizeof (:'a) (ArrayT t n) = n * sizeof (:'a) t) ∧
-  (sizeof (:'a) (TupleT ts) = sum (map (sizeof (:'a)) ts))
+  (sizeof (IntegerT n) = (n+7) DIV 8) ∧
+  (sizeof (PointerT t) = (pointer_size+7) DIV 8) ∧
+  (sizeof (ArrayT t n) = n * sizeof t) ∧
+  (sizeof (TupleT ts) = sum (map sizeof ts))
 Termination
-  WF_REL_TAC `measure (typ_size o snd)` >> simp [] >>
+  WF_REL_TAC `measure typ_size` >> simp [] >>
   Induct >> rw [definition "typ_size_def"] >> simp [] >>
   first_x_assum drule >> decide_tac
-End
-
-Definition type_to_shape_def:
-  (type_to_shape (:'a) (IntegerT n) = Flat (sizeof (:'a) (IntegerT n)) (IntegerT n)) ∧
-  (type_to_shape (:'a) (ArrayT t n) = Array (type_to_shape (:'a) t) n) ∧
-  (type_to_shape (:'a) (TupleT ts) = Tuple (map (type_to_shape (:'a)) ts))
-Termination
-  WF_REL_TAC `measure (typ_size o snd)` >>
-  rw [] >>
-  Induct_on `ts` >> rw [definition "typ_size_def"] >>
-  res_tac >> decide_tac
 End
 
 Definition first_class_type_def:
@@ -185,34 +178,53 @@ Termination
 End
 
 Inductive value_type:
-  (value_type (IntegerT n) (FlatV (IntV i n))) ∧
-  (value_type (PointerT _) (FlatV (LocV n))) ∧
-  (every (value_type t) vs ∧ length vs = n ∧ first_class_type t
+  (∀n i. value_type (IntegerT n) (FlatV (IntV i n))) ∧
+  (∀t vs n.
+   every (value_type t) vs ∧ length vs = n ∧ first_class_type t
    ⇒
    value_type (ArrayT t n) (AggV vs)) ∧
-  (list_rel value_type ts vs
+  (∀ts vs.
+   list_rel value_type ts vs
    ⇒
-   value_type (StrT ts) (AggV vs))
+   value_type (TupleT ts) (AggV vs))
 End
 
 Definition bool2v_def:
   bool2v b = FlatV (IntV (if b then 1 else 0) 1)
 End
 
-Definition int2unsigned_def:
-  int2unsigned (i:int) size =
+(* The integer, interpreted as 2's complement, fits in the given number of bits *)
+Definition ifits_def:
+  ifits (i:int) size ⇔
+    0 < size ∧ -(2 ** (size - 1)) ≤ i ∧ i < 2 ** (size - 1)
+End
+
+(* The natural number, interpreted as unsigned, fits in the given number of bits *)
+Definition nfits_def:
+  nfits (n:num) size ⇔
+    0 < size ∧ n < 2 ** size
+End
+
+(* Convert an integer to an unsigned number, following the 2's complement,
+ * assuming (ifits i size) *)
+Definition i2n_def:
+  i2n (IntV i size) : num =
     if i < 0 then
-      256 ** size + i
+      Num (2 ** size + i)
     else
-      i
+      Num i
 End
 
-Definition fits_def:
-  fits (i:int) size ⇔
-    0 < size ∧ 0 - (256 ** (size - 1)) ≤ i ∧ i < 256 ** (size - 1)
+(* Convert an unsigned number into the integer that it would be in 2's
+ * compliment with the given size, assuming (nfits n size) *)
+Definition n2i_def:
+  n2i n size =
+    if 2 ** (size - 1) ≤ n then
+      (IntV (&n - &(2 ** size)) size)
+    else
+      (IntV (&n) size)
 End
 
-(* TODO: We never create anything that is a SizeV *)
 Inductive eval_exp:
   (∀s v r.
    flookup s.locals v = Some r
@@ -222,17 +234,19 @@ Inductive eval_exp:
   (* TODO: Nondet I guess we need to know the type here *)
   (* TODO: Label *)
 
-  (∀s e1 e2 size byte.
-   eval_exp s e1 (FlatV (IntV byte 1)) ∧
-   eval_exp s e2 (FlatV (SizeV size))
+  (∀s e1 e2 n byte n_size.
+   eval_exp s e1 (FlatV (IntV byte 8)) ∧
+   (* This idiom means that e2 evaluates to a non-negative integer n, and is
+    * used throughout *)
+   eval_exp s e2 (FlatV (IntV (&n) n_size))
    ⇒
-   eval_exp s (Splat e1 e2) (AggV (replicate size (FlatV (IntV byte 1))))) ∧
+   eval_exp s (Splat e1 e2) (AggV (replicate n (FlatV (IntV byte 8))))) ∧
 
    (* TODO Question: What if size <> vals? *)
-  (∀s e1 e2 size vals.
+  (∀s e1 e2 l vals n_size.
    eval_exp s e1 (AggV vals) ∧
-   eval_exp s e2 (FlatV (SizeV size)) ∧
-   size = length vals
+   eval_exp s e2 (FlatV (IntV (&l) n_size)) ∧
+   l = length vals
    ⇒
    eval_exp s (Memory e1 e2) (AggV vals)) ∧
 
@@ -242,7 +256,7 @@ Inductive eval_exp:
    eval_exp s (Concat es) (AggV (flat vals))) ∧
 
   (∀s i size.
-   eval_exp s (Integer i (IntegerT size)) (FlatV (IntV i size))) ∧
+   eval_exp s (Integer i (IntegerT size)) (FlatV (IntV (truncate_2comp i size) size))) ∧
 
   (* TODO Question: Should the same integer with two different sizes be equal *)
   (∀s e1 e2 r1 r2.
@@ -254,136 +268,146 @@ Inductive eval_exp:
   (∀s e1 e2 i1 size1 i2 size2.
    eval_exp s e1 (FlatV (IntV i1 size1)) ∧
    eval_exp s e2 (FlatV (IntV i2 size2)) ∧
-   fits i1 size1 ∧
-   fits i2 size2
+   ifits i1 size1 ∧
+   ifits i2 size2
    ⇒
    eval_exp s (Lt e1 e2) (bool2v (i1 < i2))) ∧
 
-  (∀s e1 e2 i1 size1 i2 size2.
+  (∀s e1 e2 i1 i2 size1 size2.
    eval_exp s e1 (FlatV (IntV i1 size1)) ∧
    eval_exp s e2 (FlatV (IntV i2 size2)) ∧
-   fits i1 size1 ∧
-   fits i2 size2
+   ifits i1 size1 ∧
+   ifits i2 size2
    ⇒
-   eval_exp s (Ult e1 e2) (bool2v (int2unsigned i1 size1 < int2unsigned i2 size2))) ∧
+   eval_exp s (Ult e1 e2) (bool2v (i2n (IntV i1 size1) < i2n (IntV i2 size2)))) ∧
 
   (∀s size e1 e2 i1 i2.
    eval_exp s e1 (FlatV (IntV i1 size)) ∧
-   eval_exp s e2 (FlatV (IntV i2 size)) ∧
-   fits i1 size ∧
-   fits i2 size
+   eval_exp s e2 (FlatV (IntV i2 size))
    ⇒
-   eval_exp s (Sub (IntegerT size) e1 e2) (FlatV (IntV (i1 - i2) size))) ∧
+   eval_exp s (Sub (IntegerT size) e1 e2) (FlatV (IntV (truncate_2comp (i1 - i2) size) size))) ∧
 
   (∀s es vals.
    list_rel (eval_exp s) es vals
    ⇒
    eval_exp s (Record es) (AggV vals)) ∧
 
-  (∀s e1 e2 vals size.
+  (∀s e1 e2 vals idx idx_size.
    eval_exp s e1 (AggV vals) ∧
-   eval_exp s e2 (FlatV (SizeV size)) ∧
-   size < length vals
+   eval_exp s e2 (FlatV (IntV (&idx) idx_size)) ∧
+   idx < length vals
    ⇒
-   eval_exp s (Select e1 e2) (el size vals)) ∧
+   eval_exp s (Select e1 e2) (el idx vals)) ∧
 
-  (∀s e1 e2 e3 vals size r.
+  (∀s e1 e2 e3 vals r idx idx_size.
    eval_exp s e1 (AggV vals) ∧
-   eval_exp s e2 (FlatV (SizeV size)) ∧
+   eval_exp s e2 (FlatV (IntV (&idx) idx_size)) ∧
    eval_exp s e3 r ∧
-   size < length vals
+   idx < length vals
    ⇒
-   eval_exp s (Update e1 e2 e3) (AggV (list_update r size vals)))
+   eval_exp s (Update e1 e2 e3) (AggV (list_update r idx vals)))
 
+End
+
+(* BEGIN Functions to interface to the generic memory model *)
+Definition type_to_shape_def:
+  (type_to_shape (IntegerT n) = Flat (sizeof (IntegerT n)) (IntegerT n)) ∧
+  (type_to_shape (ArrayT t n) = Array (type_to_shape t) n) ∧
+  (type_to_shape (TupleT ts) = Tuple (map type_to_shape ts))
+Termination
+  WF_REL_TAC `measure typ_size` >>
+  rw [] >>
+  Induct_on `ts` >> rw [definition "typ_size_def"] >>
+  res_tac >> decide_tac
 End
 
 Definition convert_value_def:
-  (convert_value (IntegerT n) w = IntV (w2i w) n) ∧
-  (convert_value (PointerT t) w = LocV (w2n w))
+  convert_value (IntegerT size) n = IntV (&n) size
 End
 
 Definition bytes_to_llair_value_def:
-  bytes_to_llair_value (:'a) t bs =
-    (bytes_to_value (λn t (w:'a word). convert_value t w) (type_to_shape (:'a) t) bs)
+  bytes_to_llair_value t bs =
+    (bytes_to_value (λn t w. convert_value t w) (type_to_shape t) bs)
 End
 
 Definition unconvert_value_def:
-  (unconvert_value (:'a) (IntV i size) = (size, i2w i)) ∧
-  (unconvert_value (:'a) (LocV n) = (dimindex (:'a), n2w n))
+  unconvert_value (IntV i size) = ((size + 7) DIV 8, i2n (IntV i size))
 End
 
 Definition llair_value_to_bytes_def:
-  llair_value_to_bytes (:'a) v =
-    value_to_bytes (unconvert_value (:'a) : flat_v -> num # 'a word) v
+  llair_value_to_bytes v =
+    value_to_bytes unconvert_value v
 End
+(* END Functions to interface to the generic memory model *)
 
 Definition update_results_def:
   update_results xvs s = s with locals := s.locals |++ xvs
 End
 
 Inductive step_inst:
-  (∀s ves r.
-    eval_exp s e r
+  (∀s ves rs.
+    list_rel (eval_exp s) (map snd ves) rs
     ⇒
     step_inst s
     (Move ves)
-    (update_results (map (λ(v,e). (v, r)) ves) s)) ∧
+    (update_results (map (λ(v,r). (v, r)) (zip (map fst ves, rs))) s)) ∧
 
-  (∀(s:'a state) x t e size ptr freeable interval bytes.
-   eval_exp s e (FlatV (LocV ptr)) ∧
-   interval = Interval freeable ptr (ptr + size) ∧
+  (∀s x t e size ptr freeable interval bytes.
+   eval_exp s e (FlatV ptr) ∧
+   interval = Interval freeable (i2n ptr) (i2n ptr + size) ∧
    is_allocated interval s.heap ∧
    bytes = map snd (get_bytes s.heap interval)
    ⇒
    step_inst s
     (Load (Var_name x t) e size)
-    (update_results [(Var_name x t, fst (bytes_to_llair_value (:'a) t bytes))] s)) ∧
+    (update_results [(Var_name x t, fst (bytes_to_llair_value t bytes))] s)) ∧
 
   (∀s e1 e2 size ptr bytes freeable interval r.
-   eval_exp s e1 (FlatV (LocV ptr)) ∧
+   eval_exp s e1 (FlatV ptr) ∧
    eval_exp s e2 r ∧
-   interval = Interval freeable ptr (ptr + size) ∧
+   interval = Interval freeable (i2n ptr) (i2n ptr + size) ∧
    is_allocated interval s.heap ∧
-   bytes = llair_value_to_bytes (:'a) r ∧
+   bytes = llair_value_to_bytes r ∧
    length bytes = size
    ⇒
    step_inst s
      (Store e1 e2 size)
-     (s with heap := set_bytes () bytes ptr s.heap)) ∧
+     (s with heap := set_bytes () bytes (i2n ptr) s.heap)) ∧
 
   (* TODO memset *)
 
   (∀s e1 e2 e3 dest_ptr src_ptr size src_interval freeable1 freeable2 bytes.
-   eval_exp s e1 (FlatV (LocV dest_ptr)) ∧
-   eval_exp s e2 (FlatV (LocV src_ptr)) ∧
-   eval_exp s e3 (FlatV (SizeV size)) ∧
-   src_interval = Interval freeable1 src_ptr (src_ptr + size) ∧
+   eval_exp s e1 (FlatV dest_ptr) ∧
+   eval_exp s e2 (FlatV src_ptr) ∧
+   eval_exp s e3 (FlatV size) ∧
+   src_interval = Interval freeable1 (i2n src_ptr) (i2n src_ptr + i2n size) ∧
    is_allocated src_interval s.heap ∧
-   is_allocated (Interval freeable2 dest_ptr (dest_ptr + size)) s.heap ∧
+   is_allocated (Interval freeable2 (i2n dest_ptr) (i2n dest_ptr + i2n size)) s.heap ∧
    (* TODO Question: should we allow overlap? *)
    bytes = map snd (get_bytes s.heap src_interval)
    ⇒
    step_inst s
     (Memcpy e1 e2 e3)
-    (s with heap := set_bytes () bytes dest_ptr s.heap)) ∧
+    (s with heap := set_bytes () bytes (i2n dest_ptr) s.heap)) ∧
 
   (* TODO memmove *)
 
-  (∀s v e1 e2 n size ptr new_h.
-   eval_exp s e1 (FlatV (SizeV n)) ∧
-   eval_exp s e2 (FlatV (SizeV size)) ∧
-   allocate s.heap (n * size) () (ptr, new_h)
+  (∀s v e1 e2 n size ptr new_h size_size.
+   eval_exp s e1 (FlatV n) ∧
+   eval_exp s e2 (FlatV (IntV (&size) size_size)) ∧
+   allocate s.heap (i2n n * size) () (ptr, new_h) ∧
+   nfits ptr pointer_size
    ⇒
    step_inst s
      (Alloc v e1 e2)
-     (update_results [(v, FlatV (LocV ptr))] (s with heap := new_h))) ∧
+     (update_results [(v, FlatV (n2i ptr pointer_size))] (s with heap := new_h))) ∧
 
   (∀s e ptr.
-   eval_exp s e (FlatV (LocV ptr))
+   eval_exp s e (FlatV ptr)
    ⇒
    step_inst s
      (Free e)
-     (s with heap := deallocate [A ptr] s.heap)) ∧
+     (s with heap := deallocate [A (i2n ptr)] s.heap)) ∧
 
   (∀s x t nondet.
    value_type t nondet
@@ -396,22 +420,22 @@ End
 
 Inductive step_term:
 
-  (∀prog s e table default size fname bname bname'.
-   eval_exp s e (FlatV (SizeV size)) ∧
-   Lab_name fname bname = (case alookup table size of Some lab => lab | None => default) ∧
+  (∀prog s e table default idx fname bname bname' idx_size.
+   eval_exp s e (FlatV (IntV (&idx) idx_size)) ∧
+   Lab_name fname bname = (case alookup table idx of Some lab => lab | None => default) ∧
    s.bp = Lab_name fname bname'
    ⇒
    step_term prog s
      (Switch e table default)
      (s with bp := Lab_name fname bname)) ∧
 
-  (∀prog s e labs size.
-   eval_exp s e (FlatV (SizeV size)) ∧
-   size < length labs
+  (∀prog s e labs i idx idx_size.
+   eval_exp s e (FlatV (IntV (&idx) idx_size)) ∧
+   idx < length labs
    ⇒
    step_term prog s
      (Iswitch e labs)
-     (s with bp := el size labs)) ∧
+     (s with bp := el i labs)) ∧
 
   (∀prog s v fname bname es t ret1 ret2 vals f.
    alookup prog.functions fname = Some f ∧
@@ -428,7 +452,6 @@ Inductive step_term:
              exn_ret := ret2;
              ret_var := v;
              saved_locals := s.locals |> :: s.stack;
-        pointer_size := s.pointer_size;
         heap := s.heap |>) ∧
 
   (∀prog s e r top rest.
@@ -441,7 +464,6 @@ Inductive step_term:
         globals := s.globals;
         locals := top.saved_locals |+ (top.ret_var, r);
         stack := rest;
-        pointer_size := s.pointer_size;
         heap := s.heap |>)
 
   (* TODO Throw *)
@@ -452,12 +474,12 @@ End
  * instruction pointer and do a big-step evaluation for each block *)
 Inductive step_block:
 
-  (!prog s1 t s2.
+  (∀prog s1 t s2.
    step_term prog s1 t s2
    ⇒
    step_block prog s1 [] t s2) ∧
 
-  (!prog s1 i is t s2 s3.
+  (∀prog s1 i is t s2 s3.
    step_inst s1 i s2 ∧
    step_block prog s2 is t s3
    ⇒
