sledge/semantics/llvmScript.sml
@@ -136,12 +136,17 @@ End
 
 (* ----- Semantic states ----- *)
 
+Definition pointer_size_def:
+  pointer_size = 8
+End
+
 Datatype:
   flat_v =
   | W1V word1
   | W8V word8
   | W32V word32
   | W64V word64
+  (* LLVM guarantees that 64 bits is enough to hold a pointer *)
   | PtrV word64
   | UndefV
 End
@@ -172,13 +177,21 @@ End
 
 (* ----- Things about types ----- *)
 
+(* Given a number n that fits into pointer_size number of bytes, create the
+ * pointer value. Since the pointer is represented as a 64-bit word,
+ * pointer_size must be 8 or less, which LLVM guarantees *)
+Definition mk_ptr_def:
+  mk_ptr n =
+    if n < 256 ** pointer_size then Some (FlatV (PtrV (n2w n))) else None
+End
+
 (* How many bytes a value of the given type occupies *)
 Definition sizeof_def:
   (sizeof (IntT W1) = 1) ∧
   (sizeof (IntT W8) = 1) ∧
   (sizeof (IntT W32) = 4) ∧
   (sizeof (IntT W64) = 8) ∧
-  (sizeof (PtrT _) = 8) ∧
+  (sizeof (PtrT _) = pointer_size) ∧
   (sizeof (ArrT n t) = n * sizeof t) ∧
   (sizeof (StrT ts) = sum (map sizeof ts))
 Termination
@@ -200,6 +213,7 @@ Termination
   res_tac >> decide_tac
 End
 
+(* Are the indices all in bounds? *)
 Definition indices_ok_def:
   (indices_ok _ [] ⇔ T) ∧
   (indices_ok (ArrT n t) (i::indices) ⇔
@@ -209,12 +223,13 @@ Definition indices_ok_def:
   (indices_ok _ _ ⇔ F)
 End
 
+(* Which values have which types *)
 Inductive value_type:
   (value_type (IntT W1) (FlatV (W1V w1))) ∧
   (value_type (IntT W8) (FlatV (W8V w8))) ∧
   (value_type (IntT W32) (FlatV (W32V w32))) ∧
   (value_type (IntT W64) (FlatV (W64V w64))) ∧
-  (value_type (PtrT _) (FlatV (PtrV w64))) ∧
+  (value_type (PtrT _) (FlatV (PtrV ptr))) ∧
   (every (value_type t) vs ∧ length vs = n ∧ first_class_type t
    ⇒
    value_type (ArrT n t) (AggV vs)) ∧
@@ -223,6 +238,7 @@ Inductive value_type:
    value_type (StrT ts) (AggV vs))
 End
 
+(* Get the component of a type referred by the indices *)
 Definition extract_type_def:
   (extract_type t [] = Some t) ∧
   (extract_type (ArrT n t) (i::idx) =
@@ -257,6 +273,7 @@ End
 
 (* ----- Semantic transitions ----- *)
 
+(* Put a 64-bit word into a smaller value, truncating if necessary *)
 Definition w64_cast_def:
   (w64_cast w (IntT W1) = Some (FlatV (W1V (w2w w)))) ∧
   (w64_cast w (IntT W8) = Some (FlatV (W8V (w2w w)))) ∧
@@ -265,22 +282,37 @@ Definition w64_cast_def:
   (w64_cast _ _ = None)
 End
 
-Definition cast_w64_def:
-  (cast_w64 (FlatV (W1V w)) = Some (w2w w)) ∧
-  (cast_w64 (FlatV (W8V w)) = Some (w2w w)) ∧
-  (cast_w64 (FlatV (W32V w)) = Some (w2w w)) ∧
-  (cast_w64 (FlatV (W64V w)) = Some w) ∧
-  (cast_w64 _ = None)
-End
-
-Definition cast_num_def:
-  cast_num v = option_map w2n (cast_w64 v)
-End
-
 Definition bool_to_v_def:
   bool_to_v b = if b then FlatV (W1V 1w) else FlatV (W1V 0w)
 End
 
+(* Convert a word value into an integer, interpreting the word in 2's complement *)
+Definition signed_v_to_int_def:
+  (signed_v_to_int (FlatV (W1V w)) = Some (w2i w)) ∧
+  (signed_v_to_int (FlatV (W8V w)) = Some (w2i w)) ∧
+  (signed_v_to_int (FlatV (W32V w)) = Some (w2i w)) ∧
+  (signed_v_to_int (FlatV (W64V w)) = Some (w2i w)) ∧
+  (signed_v_to_int _ = None)
+End
+
+(* Convert a non-negative word value (interpreted as 2's complement) into a natural number *)
+Definition signed_v_to_num_def:
+  signed_v_to_num v =
+    option_join
+      (option_map (\i. if i < 0 then None else Some (Num i)) (signed_v_to_int v))
+End
+
+(* Convert a word value into a natural number, interpreting the word as unsigned *)
+Definition unsigned_v_to_num_def:
+  (unsigned_v_to_num (FlatV (W1V w)) = Some (w2n w)) ∧
+  (unsigned_v_to_num (FlatV (W8V w)) = Some (w2n w)) ∧
+  (unsigned_v_to_num (FlatV (W32V w)) = Some (w2n w)) ∧
+  (unsigned_v_to_num (FlatV (W64V w)) = Some (w2n w)) ∧
+  (unsigned_v_to_num _ = None)
+End
+
+(* TODO: This is a bit of a mess. Consider changing to a relation to deal with
+ * partiality *)
 Definition eval_const_def:
   (eval_const g (IntC W1 i) = FlatV (W1V (i2w i))) ∧
   (eval_const g (IntC W8 i) = FlatV (W8V (i2w i))) ∧
@@ -289,12 +321,12 @@ Definition eval_const_def:
   (eval_const g (StrC tconsts) = AggV (map (eval_const g) (map snd tconsts))) ∧
   (eval_const g (ArrC tconsts) = AggV (map (eval_const g) (map snd tconsts))) ∧
   (eval_const g (GepC ty ptr (t, idx) indices) =
-    case (eval_const g ptr, cast_num (eval_const g idx)) of
-    | (FlatV (PtrV w), Some n) =>
-      let ns = map (λ(t,ci). case cast_num (eval_const g ci) of None => 0 | Some n => n) indices in
+    case (eval_const g ptr, signed_v_to_num (eval_const g idx)) of
+    | (FlatV (PtrV ptr), Some n) =>
+      let ns = map (λ(t,ci). case signed_v_to_num (eval_const g ci) of None => 0 | Some n => n) indices in
         (case get_offset ty ns of
          | None => FlatV UndefV
-         | Some off => FlatV (PtrV (n2w (w2n w + sizeof ty * n + off))))
+         | Some off => FlatV (PtrV (n2w ((w2n ptr) + (sizeof ty) * n + off))))
     | _ => FlatV UndefV) ∧
   (eval_const g (GlobalC var) =
     case flookup g var of
@@ -312,21 +344,11 @@ Termination
 End
 
 Definition eval_def:
-  (eval s (Variable v) =
-    case flookup s.locals v of
-    | None => <| poison := F; value := FlatV (W1V 0w) |>
-    | Some v => v) ∧
-  (eval s (Constant c) = <| poison := F; value := eval_const s.globals c |>)
+  (eval s (Variable v) = flookup s.locals v) ∧
+  (eval s (Constant c) = Some <| poison := F; value := eval_const s.globals c |>)
 End
 
-Definition v2n_def:
-  (v2n (FlatV (W1V b)) = Some (if T then 1 else 0)) ∧
-  (v2n (FlatV (W8V w8)) = Some (w2n w8)) ∧
-  (v2n (FlatV (W32V w32)) = Some (w2n w32)) ∧
-  (v2n (FlatV (W64V w64)) = Some (w2n w64)) ∧
-  (v2n _ = None)
-End
-
+(* BEGIN Functions to interface to the generic memory model *)
 Definition type_to_shape_def:
   (type_to_shape (IntT s) = Flat (sizeof (IntT s)) (IntT s)) ∧
   (type_to_shape (PtrT t) = Flat (sizeof (PtrT t)) (PtrT t)) ∧
@@ -339,11 +361,11 @@ Termination
 End
 
 Definition convert_value_def:
-  (convert_value (IntT W1) w = W1V (w2w w)) ∧
-  (convert_value (IntT W8) w = W8V (w2w w)) ∧
-  (convert_value (IntT W32) w = W32V (w2w w)) ∧
-  (convert_value (IntT W64) w = W64V w) ∧
-  (convert_value (PtrT _) w = PtrV w)
+  (convert_value (IntT W1) n = W1V (n2w n)) ∧
+  (convert_value (IntT W8) n = W8V (n2w n)) ∧
+  (convert_value (IntT W32) n = W32V (n2w n)) ∧
+  (convert_value (IntT W64) n = W64V (n2w n)) ∧
+  (convert_value (PtrT _) n = PtrV (n2w n))
 End
 
 Definition bytes_to_llvm_value_def:
@@ -352,11 +374,11 @@ Definition bytes_to_llvm_value_def:
 End
 
 Definition unconvert_value_def:
-  (unconvert_value (W1V w) = (1, w2w w)) ∧
-  (unconvert_value (W8V w) = (1, w2w w)) ∧
-  (unconvert_value (W32V w) = (4, w2w w)) ∧
-  (unconvert_value (W64V w) = (8, w)) ∧
-  (unconvert_value (PtrV w) = (8, w))
+  (unconvert_value (W1V w) = (1, w2n w)) ∧
+  (unconvert_value (W8V w) = (1, w2n w)) ∧
+  (unconvert_value (W32V w) = (4, w2n w)) ∧
+  (unconvert_value (W64V w) = (8, w2n w)) ∧
+  (unconvert_value (PtrV w) = (pointer_size, w2n w))
 End
 
 Definition llvm_value_to_bytes_def:
@@ -364,17 +386,27 @@ Definition llvm_value_to_bytes_def:
     value_to_bytes unconvert_value v
 End
 
+(* END Functions to interface to the generic memory model *)
+
 Definition do_sub_def:
-  do_sub (nuw:bool) (nsw:bool) (v1:pv) (v2:pv) =
-    let (diff, u_overflow, s_overflow) =
-      case (v1.value, v2.value) of
-      | (FlatV (W1V w1), FlatV (W1V w2)) => (FlatV o W1V ## I) (add_with_carry (w1, ¬w2, T))
-      | (FlatV (W8V w1), FlatV (W8V w2)) => (FlatV o W8V ## I) (add_with_carry (w1, ¬w2, T))
-      | (FlatV (W32V w1), FlatV (W32V w2)) => (FlatV o W32V ## I) (add_with_carry (w1, ¬w2, T))
-      | (FlatV (W64V w1), FlatV (W64V w2)) => (FlatV o W64V ## I) (add_with_carry (w1, ¬w2, T))
+  do_sub (nuw:bool) (nsw:bool) (v1:pv) (v2:pv) t =
+    let diff =
+      case (v1.value, v2.value, t) of
+      | (FlatV (W1V w1), FlatV (W1V w2), IntT W1) =>
+        Some ((FlatV o W1V ## I) (add_with_carry (w1, ¬w2, T)))
+      | (FlatV (W8V w1), FlatV (W8V w2), IntT W8) =>
+        Some ((FlatV o W8V ## I) (add_with_carry (w1, ¬w2, T)))
+      | (FlatV (W32V w1), FlatV (W32V w2), IntT W32) =>
+        Some ((FlatV o W32V ## I) (add_with_carry (w1, ¬w2, T)))
+      | (FlatV (W64V w1), FlatV (W64V w2), IntT W64) =>
+        Some ((FlatV o W64V ## I) (add_with_carry (w1, ¬w2, T)))
+      | _ => None
     in
-    let p = ((nuw ∧ u_overflow) ∨ (nsw ∧ s_overflow) ∨ v1.poison ∨ v2.poison) in
-      <| poison := p; value := diff |>
+      option_map
+        (\(diff, u_overflow, s_overflow).
+           let p = ((nuw ∧ u_overflow) ∨ (nsw ∧ s_overflow) ∨ v1.poison ∨ v2.poison) in
+             <| poison := p; value := diff |>)
+        diff
 End
 
 Definition get_comp_def:
@@ -385,19 +417,19 @@ End
 
 Definition do_icmp_def:
   do_icmp c v1 v2 =
-    <| poison := (v1.poison ∨ v2.poison);
-       value := bool_to_v (
-         case (v1.value, v2.value) of
-         | (FlatV (W1V w1), FlatV (W1V w2)) => (get_comp c) w1 w2
-         | (FlatV (W8V w1), FlatV (W8V w2)) => (get_comp c) w1 w2
-         | (FlatV (W32V w1), FlatV (W32V w2)) => (get_comp c) w1 w2
-         | (FlatV (W64V w1), FlatV (W64V w2)) => (get_comp c) w1 w2
-         | (FlatV (PtrV w1), FlatV (PtrV w2)) => (get_comp c) w1 w2) |>
+    option_map (\b. <| poison := (v1.poison ∨ v2.poison); value := bool_to_v b |>)
+      (case (v1.value, v2.value) of
+       | (FlatV (W1V w1), FlatV (W1V w2)) => Some ((get_comp c) w1 w2)
+       | (FlatV (W8V w1), FlatV (W8V w2)) => Some ((get_comp c) w1 w2)
+       | (FlatV (W32V w1), FlatV (W32V w2)) => Some ((get_comp c) w1 w2)
+       | (FlatV (W64V w1), FlatV (W64V w2)) => Some ((get_comp c) w1 w2)
+       | (FlatV (PtrV w1), FlatV (PtrV w2)) => Some ((get_comp c) w1 w2)
+       | _ => None)
 End
 
 Definition do_phi_def:
   do_phi from_l s (Phi id _ entries) =
-    option_map (λarg. (id, eval s arg)) (alookup entries from_l)
+    option_join (option_map (λarg. option_map (\v. (id, v)) (eval s arg)) (alookup entries from_l))
 End
 
 Definition extract_value_def:
@@ -436,11 +468,12 @@ End
 Inductive step_instr:
 
   (s.stack = fr::st ∧
-   deallocate fr.stack_allocs s.heap = new_h
+   deallocate fr.stack_allocs s.heap = new_h ∧
+   eval s a = Some v
    ⇒
    step_instr prog s
      (Ret (t, a))
-     (update_result fr.result_var (eval s a)
+     (update_result fr.result_var v
        <| ip := fr.ret;
           globals := s.globals;
           locals := fr.saved_locals;
@@ -458,7 +491,7 @@ Inductive step_instr:
  * %r2 = phi [%r1, %l]
  * %r1 = phi [0, %l]
  *)
-  (eval s a = <| poison := p; value := FlatV (W1V tf) |> ∧
+  (eval s a = Some <| poison := p; value := FlatV (W1V tf) |> ∧
    l = Some (if tf = 1w then l1 else l2) ∧
    alookup prog s.ip.f = Some d ∧
    alookup d.blocks l = Some <| h := Head phis None; body := b |> ∧
@@ -472,22 +505,29 @@ Inductive step_instr:
   (* TODO *)
   (step_instr prog s (Invoke r t a args l1 l2) s) ∧
 
-  (step_instr prog s
+  (eval s a1 = Some v1 ∧
+   eval s a2 = Some v2 ∧
+   do_sub nuw nsw v1 v2 t = Some v3
+   ⇒
+   step_instr prog s
      (Sub r nuw nsw t a1 a2)
-     (inc_pc (update_result r (do_sub nuw nsw (eval s a1) (eval s a2)) s))) ∧
+     (inc_pc (update_result r v3 s))) ∧
 
-  (eval s a = v ∧
-   map (λci. cast_num (eval_const s.globals ci)) const_indices = map Some ns ∧
+  (eval s a = Some v ∧
+   (* The manual implies (but does not explicitly state) that the indices are
+    * interpreted as signed numbers *)
+   map (λci. signed_v_to_num (eval_const s.globals ci)) const_indices = map Some ns ∧
    extract_value v.value ns = Some result
    ⇒
    step_instr prog s
      (Extractvalue r (t, a) const_indices)
-     (inc_pc (update_result r
-                <| poison := v.poison; value := result |> s))) ∧
+     (inc_pc (update_result r <| poison := v.poison; value := result |> s))) ∧
 
-  (eval s a1 = v1 ∧
-   eval s a2 = v2 ∧
-   map (λci. cast_num (eval_const s.globals ci)) const_indices = map Some ns ∧
+  (eval s a1 = Some v1 ∧
+   eval s a2 = Some v2 ∧
+   (* The manual implies (but does not explicitly state) that the indices are
+    * interpreted as signed numbers *)
+   map (λci. signed_v_to_num (eval_const s.globals ci)) const_indices = map Some ns ∧
    insert_value v1.value v2.value ns = Some result
    ⇒
    step_instr prog s
@@ -495,16 +535,19 @@ Inductive step_instr:
      (inc_pc (update_result r
                 <| poison := (v1.poison ∨ v2.poison); value := result |> s))) ∧
 
-  (eval s a1 = v ∧
-   v2n v.value = Some n ∧
-   allocate s.heap (n * sizeof t) v.poison (n2, new_h)
+  (eval s a1 = Some v ∧
+   (* TODO Question is the number to allocate interpreted as a signed or
+    * unsigned quantity. E.g., if we allocate i8 0xFF does that do 255 or -1? *)
+   signed_v_to_num v.value = Some n ∧
+   allocate s.heap (n * sizeof t) v.poison (n2, new_h) ∧
+   mk_ptr n2 = Some ptr
    ⇒
    step_instr prog s
      (Alloca r t (t1, a1))
-     (inc_pc (update_result r <| poison := v.poison; value := FlatV (PtrV (n2w n2)) |>
+     (inc_pc (update_result r <| poison := v.poison; value := ptr |>
                 (s with heap := new_h)))) ∧
 
-  (eval s a1 = <| poison := p1; value := FlatV (PtrV w) |> ∧
+  (eval s a1 = Some <| poison := p1; value := FlatV (PtrV w) |> ∧
    interval = Interval freeable (w2n w) (w2n w + sizeof t) ∧
    is_allocated interval s.heap ∧
    pbytes = get_bytes s.heap interval
@@ -515,30 +558,34 @@ Inductive step_instr:
                                  value := fst (bytes_to_llvm_value t (map snd pbytes)) |>
                             s))) ∧
 
-  (eval s a2 = <| poison := p2; value := FlatV (PtrV w) |> ∧
+  (eval s a2 = Some <| poison := p2; value := FlatV (PtrV w) |> ∧
+   eval s a1 = Some v1 ∧
    interval = Interval freeable (w2n w) (w2n w + sizeof t) ∧
    is_allocated interval s.heap ∧
-   bytes = llvm_value_to_bytes (eval s a1).value ∧
+   bytes = llvm_value_to_bytes v1.value ∧
    length bytes = sizeof t
    ⇒
    step_instr prog s
      (Store (t1, a1) (t2, a2))
      (inc_pc (s with heap := set_bytes p2 bytes (w2n w) s.heap))) ∧
 
-  (map (eval s o snd) tindices = i1::indices ∧
-   (eval s a1).value = FlatV (PtrV w1) ∧
-   cast_num i1.value = Some n ∧
-   map (λx. cast_num x.value) indices = map Some ns ∧
-   get_offset t1 ns = Some off
+  (map (eval s o snd) tindices = map Some (i1::indices) ∧
+   eval s a1 = Some v ∧
+   v.value = FlatV (PtrV w1) ∧
+   (* The manual states that the indices are interpreted as signed numbers *)
+   signed_v_to_num i1.value = Some i ∧
+   map (λx. signed_v_to_num x.value) indices = map Some is ∧
+   get_offset t1 is = Some off ∧
+   mk_ptr (w2n w1 + sizeof t1 * i + off) = Some ptr
    ⇒
    step_instr prog s
     (Gep r t ((PtrT t1), a1) tindices)
     (inc_pc (update_result r
                <| poison := (v1.poison ∨ i1.poison ∨ exists (λv. v.poison) indices);
-                  value := FlatV (PtrV (n2w (w2n w1 + sizeof t1 * n + off))) |>
+                  value := ptr |>
                s))) ∧
 
-  (eval s a1 = v1 ∧
+  (eval s a1 = Some v1 ∧
    v1.value = FlatV (PtrV w) ∧
    w64_cast w t = Some int_v
    ⇒
@@ -546,23 +593,29 @@ Inductive step_instr:
     (Ptrtoint r (t1, a1) t)
     (inc_pc (update_result r <| poison := v1.poison; value := int_v |> s))) ∧
 
-  (eval s a1 = v1 ∧
-   cast_w64 v1.value = Some w
+  (eval s a1 = Some v1 ∧
+   unsigned_v_to_num v1.value = Some n ∧
+   mk_ptr n = Some ptr
    ⇒
    step_instr prog s
     (Inttoptr r (t1, a1) t)
-    (inc_pc (update_result r <| poison := v1.poison; value := FlatV (PtrV w) |> s))) ∧
+    (inc_pc (update_result r <| poison := v1.poison; value := ptr |> s))) ∧
 
-  (step_instr prog s
+  (eval s a1 = Some v1 ∧
+   eval s a2 = Some v2 ∧
+   do_icmp c v1 v2 = Some v3
+   ⇒
+   step_instr prog s
     (Icmp r c t a1 a2)
-    (inc_pc (update_result r (do_icmp c (eval s a1) (eval s a2)) s))) ∧
+    (inc_pc (update_result r v3 s))) ∧
 
-  (alookup prog fname = Some d
+  (alookup prog fname = Some d ∧
+   map (eval s o snd) targs = map Some vs
    ⇒
    step_instr prog s
      (Call r t fname targs)
      <| ip := <| f := fname; b := None; i := 0 |>;
-        locals := alist_to_fmap (zip (map snd d.params, map (eval s o snd) targs));
+        locals := alist_to_fmap (zip (map snd d.params, vs));
         globals := s.globals;
         stack :=
           <| ret := s.ip with i := s.ip.i + 1;
@@ -663,7 +716,7 @@ Definition is_init_state_def:
     globals_ok s ∧
     heap_ok s.heap ∧
     fdom s.globals = fdom global_init ∧
-    s.heap.valid_addresses =  { A n | n < dimword (:64) } ∧
+    s.heap.valid_addresses =  { A n | n < 256 ** pointer_size } ∧
     (* The initial allocations for globals are not freeable *)
     s.heap.allocations ⊆ { Interval F start stop | T } ∧
     (* The heap starts with the initial values of the globals written to their
