sledge/semantics/memory_modelScript.sml
@@ -47,6 +47,13 @@ Datatype:
             valid_addresses : addr set|>
 End
 
+Definition erase_tags_def:
+  erase_tags h =
+    <| memory := (λ(t,b). ((), b)) o_f h.memory;
+       allocations := h.allocations;
+       valid_addresses := h.valid_addresses |>
+End
+
 (* shapes statically describe the shape of a value in a register. Flat shapes
  * take a given number of bytes, Array shapes are replicated a certain number of
  * times
@@ -184,20 +191,21 @@ Definition deallocate_def:
 End
 
 
-(* Read len bytes from the list of bytes, and convert it into a word value,
+(* Read len bytes from the list of bytes, and convert it into a number,
  * little-endian encoding *)
-Definition le_read_w_def:
-  le_read_w len (bs : word8 list) =
+Definition le_read_num_def:
+  le_read_num len (bs : word8 list) =
     if length bs < len then
-      (l2w 256 (map w2n bs), [])
+      (l2n 256 (map w2n bs), [])
     else
-      (l2w 256 (map w2n (take len bs)), drop len bs)
+      (l2n 256 (map w2n (take len bs)), drop len bs)
 End
 
-(* Return len bytes that are the little-endian encoding of the argument word *)
-Definition le_write_w_def:
-  le_write_w len w =
-    let (l : word8 list) = map n2w (w2l 256 w) in
+(* Return len bytes that are the little-endian encoding of the argument number,
+ * assuming that it fits*)
+Definition le_write_num_def:
+  le_write_num len n =
+    let (l : word8 list) = map n2w (n2l 256 n) in
       take len (l ++ replicate (len - length l) 0w)
 End
 
@@ -205,7 +213,7 @@ End
  * shape. The function f is applied to the word read from a flat list of bytes
  * in little-endian order. *)
 Definition bytes_to_value_def:
-  (bytes_to_value f (Flat n t) bs = (FlatV o f n t ## I) (le_read_w n bs)) ∧
+  (bytes_to_value f (Flat n t) bs = (FlatV o f n t ## I) (le_read_num n bs)) ∧
   (bytes_to_value f (Array s n) bs = (AggV ## I) (read_array f n s bs)) ∧
   (bytes_to_value f (Tuple ts) bs = (AggV ## I) (read_str f ts bs)) ∧
   (read_array f 0 s bs = ([], bs)) ∧
@@ -230,7 +238,7 @@ End
 Definition value_to_bytes_def:
   (value_to_bytes f (FlatV x) =
     let (size, word) = f x in
-      le_write_w size word) ∧
+      le_write_num size word) ∧
   (value_to_bytes f (AggV vs) = flat (map (value_to_bytes f) vs))
 Termination
   WF_REL_TAC `measure (reg_v_size (\x. 0) o snd)` >>
@@ -241,10 +249,10 @@ End
 
 (* ----- Theorems about converting between values and byte lists ----- *)
 
-Theorem le_write_w_length:
-  ∀l x. length (le_write_w l w) = l
+Theorem le_write_num_length:
+  ∀l x. length (le_write_num l w) = l
 Proof
-  rw [le_write_w_def]
+  rw [le_write_num_def]
 QED
 
 Theorem v2b_size_lem:
@@ -255,7 +263,7 @@ Proof
   rw [value_to_bytes_def, sizeof_def, value_shape_def]
   >- (
     pairarg_tac >> simp [] >>
-    metis_tac [FST, le_write_w_length])
+    metis_tac [FST, le_write_num_length])
   >- (
     simp [LENGTH_FLAT, MAP_MAP_o, combinTheory.o_DEF] >>
     Induct_on `vs` >> rw [ADD1] >> fs [LEFT_ADD_DISTRIB] >>
@@ -271,15 +279,15 @@ Proof
 QED
 
 Theorem b2v_size_lem:
-  (∀(f:num->'c ->'a word -> 'b) s bs. sizeof s ≤ length bs ⇒
+  (∀(f:num->'c ->num -> 'b) s bs. sizeof s ≤ length bs ⇒
     ∃v. bytes_to_value f s bs = (v, drop (sizeof s) bs)) ∧
-  (∀(f:num->'c ->'a word -> 'b) n s bs. n * sizeof s ≤ length bs ⇒
+  (∀(f:num->'c ->num -> 'b) n s bs. n * sizeof s ≤ length bs ⇒
     ∃vs. read_array f n s bs = (vs, drop (n * sizeof s) bs)) ∧
-  (∀(f:num->'c ->'a word -> 'b) ss bs. sum (map sizeof ss) ≤ length bs ⇒
+  (∀(f:num->'c ->num -> 'b) ss bs. sum (map sizeof ss) ≤ length bs ⇒
     ∃vs. read_str f ss bs = (vs, drop (sum (map sizeof ss)) bs))
 Proof
   ho_match_mp_tac bytes_to_value_ind >>
-  rw [sizeof_def, bytes_to_value_def, le_read_w_def] >>
+  rw [sizeof_def, bytes_to_value_def, le_read_num_def] >>
   fs []
   >- (simp [PAIR_MAP] >> metis_tac [SND])
   >- (
@@ -305,15 +313,15 @@ Proof
 QED
 
 Theorem b2v_append_lem:
-  (∀(f:num->'c->'a word -> 'b) s bs. sizeof s ≤ length bs ⇒
+  (∀(f:num->'c->num -> 'b) s bs. sizeof s ≤ length bs ⇒
     bytes_to_value f s (bs ++ bs') = (I ## (λx. x ++ bs')) (bytes_to_value f s bs)) ∧
-  (∀(f:num->'c->'a word -> 'b) n s bs. n * sizeof s ≤ length bs ⇒
+  (∀(f:num->'c->num -> 'b) n s bs. n * sizeof s ≤ length bs ⇒
     ∃vs. read_array f n s (bs ++ bs') = (I ## (λx. x ++ bs')) (read_array f n s bs)) ∧
-  (∀(f:num->'c->'a word -> 'b) ss bs. sum (map sizeof ss) ≤ length bs ⇒
+  (∀(f:num->'c-> num -> 'b) ss bs. sum (map sizeof ss) ≤ length bs ⇒
     ∃vs. read_str f ss (bs ++ bs') = (I ## (λx. x ++ bs')) (read_str f ss bs))
 Proof
   ho_match_mp_tac bytes_to_value_ind >>
-  rw [sizeof_def, bytes_to_value_def, le_read_w_def] >>
+  rw [sizeof_def, bytes_to_value_def, le_read_num_def] >>
   fs [TAKE_APPEND, DROP_APPEND,
       DECIDE ``!x y. x ≤ y ⇒ x - y = 0n``, ETA_THM]
   >- (simp [PAIR_MAP] >> metis_tac [SND])
@@ -344,31 +352,30 @@ Proof
 QED
 
 Theorem le_read_write:
-  ∀n w bs.
-    w2n w < 256 ** n ⇒ le_read_w n (le_write_w n w ⧺ bs) = (w, bs)
+  ∀size n  bs.
+    n < 256 ** size ⇒ le_read_num size (le_write_num size n ⧺ bs) = (n, bs)
 Proof
-  rw [le_read_w_def, le_write_w_length]
+  rw [le_read_num_def, le_write_num_length]
   >- (
-    `take n (le_write_w n w ⧺ bs) = le_write_w n w`
-    by metis_tac [le_write_w_length, TAKE_LENGTH_APPEND] >>
-    simp [le_write_w_def, w2l_def, l2w_def] >>
-    Cases_on `w` >> simp [] >> fs [l2n_padding, TAKE_APPEND, take_replicate] >>
+    `take size (le_write_num size n ⧺ bs) = le_write_num size n`
+    by metis_tac [le_write_num_length, TAKE_LENGTH_APPEND] >>
+    simp [le_write_num_def, w2l_def, l2w_def] >>
+    fs [l2n_padding, TAKE_APPEND, take_replicate] >>
     simp [MAP_TAKE, MAP_MAP_o, combinTheory.o_DEF, mod_n2l] >>
     rename1 `n2l 256 m` >>
-    Cases_on `n = 0` >> fs [] >>
-    `length (n2l 256 m) ≤ n`
+    Cases_on `size = 0` >> fs [] >>
+    `length (n2l 256 m) ≤ size`
     by (
       rw [LENGTH_n2l] >>
       `256 = 2 ** 8` by EVAL_TAC >>
       ASM_REWRITE_TAC [] >> simp [log_change_base_power, GSYM LESS_EQ] >>
-      `n2w m ≠ 0w` by simp [] >>
       rw [] >> fs [bitTheory.LOG2_def, dimword_def] >>
       `8 * (log 2 m DIV 8) ≤ log 2 m` by metis_tac [mul_div_bound, EVAL ``8 ≠ 0n``] >>
-      `LOG 2 m ≤ LOG 2 (256 ** n)` by simp [LOG_LE_MONO] >>
+      `LOG 2 m ≤ LOG 2 (256 ** size)` by simp [LOG_LE_MONO, LESS_IMP_LESS_OR_EQ] >>
       pop_assum mp_tac >>
       `256 = 2 ** 8` by EVAL_TAC >>
       ASM_REWRITE_TAC [EXP_MUL] >> simp [log_base_power] >>
-      Cases_on `log 2 m DIV 8 = n` >> rw [] >>
+      Cases_on `log 2 m DIV 8 = size` >> rw [] >>
       CCONTR_TAC >> fs [] >>
       `log 2 m = (8 * (log 2 m DIV 8))` by intLib.COOPER_TAC >> fs [] >>
       `2 ** log 2 m = 2 ** (8 * (log 2 m DIV 8))` by rw [] >>
@@ -376,26 +383,24 @@ Proof
       `2 ** log 2 m ≤ m` by rw [exp_log_bound] >>
       decide_tac) >>
     simp [mod_n2l, l2n_n2l, TAKE_LENGTH_TOO_LONG])
-  >- metis_tac [le_write_w_length, DROP_LENGTH_APPEND]
+  >- metis_tac [le_write_num_length, DROP_LENGTH_APPEND]
 QED
 
 Theorem le_write_read:
-  ∀n w bs bs'.
-    256 ** n ≤ dimword (:'a) ∧
-    n ≤ length bs ∧
-    le_read_w n bs = (w:'a word, bs')
+  ∀size n bs bs'.
+    size ≤ length bs ∧
+    le_read_num size bs = (n, bs')
     ⇒
-    le_write_w n w ++ bs' = bs
+    le_write_num size n ++ bs' = bs
 Proof
-  rw [le_read_w_def] >>
-  qmatch_goalsub_abbrev_tac `l2w _ l` >>
-  `le_write_w n (l2w 256 l) = take n bs` suffices_by metis_tac [TAKE_DROP] >>
-  simp [le_write_w_def, w2l_l2w] >>
-  `l2n 256 l < 256 ** n`
+  rw [le_read_num_def] >>
+  qmatch_goalsub_abbrev_tac `l2n _ l` >>
+  `le_write_num size (l2n 256 l) = take size bs` suffices_by metis_tac [TAKE_DROP] >>
+  simp [le_write_num_def, w2l_l2w] >>
+  `l2n 256 l < 256 ** size`
   by (
-    `n ≤ length bs` by decide_tac >>
+    `size ≤ length bs` by decide_tac >>
     metis_tac [l2n_lt, LENGTH_TAKE, LENGTH_MAP, EVAL ``0n < 256``]) >>
-  fs [] >>
   `every ($> 256) l`
   by (
     simp [EVERY_MAP, Abbr `l`] >> irule EVERY_TAKE >> simp [] >>
@@ -405,15 +410,15 @@ Proof
   rw [n2l_l2n]
   >- (
     rw [TAKE_def, take_replicate] >>
-    Cases_on `n` >> fs [] >>
+    Cases_on `size` >> fs [] >>
     rfs [l2n_0] >> unabbrev_all_tac >> fs [EVERY_MAP] >>
     ONCE_REWRITE_TAC [GSYM REPLICATE] >>
-    qmatch_goalsub_abbrev_tac `take n _` >>
+    qmatch_goalsub_abbrev_tac `take size _` >>
     qpat_assum `¬(_ < _)` mp_tac >>
     qpat_assum `every (\x. 0 = w2n x) _` mp_tac >>
     rpt (pop_assum kall_tac) >>
     qid_spec_tac `bs` >>
-    Induct_on `n` >> rw [] >>
+    Induct_on `size` >> rw [] >>
     Cases_on `bs` >> rw [] >> fs [] >>
     Cases_on `h` >> fs [] >>
     first_x_assum irule >> rw [] >>
@@ -430,11 +435,11 @@ Proof
     Cases_on `l` >> fs [dropWhile_eq_nil, combinTheory.o_DEF, EXISTS_REVERSE]) >>
   `0 < length (dropWhile ($= 0) (reverse l))` by decide_tac >>
   fs [SUC_PRE] >>
-  `map n2w l = take n bs`
+  `map n2w l = take size bs`
   by (simp [Abbr `l`, MAP_TAKE, MAP_MAP_o, combinTheory.o_DEF, n2w_w2n]) >>
   simp [TAKE_TAKE_MIN] >>
-  `length l = n` by simp [Abbr `l`] >>
-  `length (dropWhile ($= 0) (reverse l)) ≤ n`
+  `length l = size` by simp [Abbr `l`] >>
+  `length (dropWhile ($= 0) (reverse l)) ≤ size`
   by metis_tac [LESS_EQ_TRANS, LENGTH_dropWhile_LESS_EQ, LENGTH_REVERSE] >>
   rw [MIN_DEF] >> fs []
   >- (
@@ -462,14 +467,14 @@ QED
 Theorem b2v_v2b_lem:
   (∀f s v.
     value_shape f s v ⇒
-    (∀x t n. f n t x ⇒ fst (h x) = n ∧ g n t (snd (h x)) = x ∧ w2n (snd (h x)) < 256 ** n) ⇒
+    (∀x t n. f n t x ⇒ fst (h x) = n ∧ g n t (snd (h x)) = x ∧ snd (h x) < 256 ** n) ⇒
     ∀bs.
-      bytes_to_value (g:num -> 'c -> 'a word -> 'b) s (value_to_bytes h v ++ bs) = (v, bs)) ∧
+      bytes_to_value g s (value_to_bytes h v ++ bs) = (v, bs)) ∧
   (∀f ss vs.
     value_shapes f ss vs ⇒
-    (∀x t n. f n t x ⇒ fst (h x) = n ∧ g n t (snd (h x)) = x ∧ w2n (snd (h x)) < 256 ** n) ⇒
+    (∀x t n. f n t x ⇒ fst (h x) = n ∧ g n t (snd (h x)) = x ∧ snd (h x) < 256 ** n) ⇒
     ∀bs.
-      read_str (g:num -> 'c -> 'a word -> 'b) ss (flat (map (value_to_bytes h) vs) ++ bs) = (vs, bs))
+      read_str g ss (flat (map (value_to_bytes h) vs) ++ bs) = (vs, bs))
 Proof
   ho_match_mp_tac value_shape_ind >> rw [value_shape_def] >>
   fs [bytes_to_value_def, value_to_bytes_def] >> rw []
@@ -501,7 +506,7 @@ QED
 Theorem b2v_v2b:
   ∀f g h s v bs.
     value_shape f s v ⇒
-    (∀x n t. f n t x ⇒ fst (h x) = n ∧ g n t (snd (h x)) = x ∧ w2n (snd (h x)) < 256 ** n) ⇒
+    (∀x n t. f n t x ⇒ fst (h x) = n ∧ g n t (snd (h x)) = x ∧ snd (h x) < 256 ** n) ⇒
       bytes_to_value g s (value_to_bytes h v ++ bs) = (v, bs)
 Proof
   metis_tac [b2v_v2b_lem]
