sledge/semantics/llair_propScript.sml
@@ -1,0 +1,141 @@
+(*
+ * Copyright (c) Facebook, Inc. and its affiliates.
+ *
+ * This source code is licensed under the MIT license found in the
+ * LICENSE file in the root directory of this source tree.
+ *)
+
+(* Properties of the llair model *)
+
+open HolKernel boolLib bossLib Parse;
+open arithmeticTheory integerTheory integer_wordTheory wordsTheory;
+open settingsTheory miscTheory llairTheory;
+
+new_theory "llair_prop";
+
+numLib.prefer_num ();
+
+Theorem ifits_w2i:
+  ∀(w : 'a word). ifits (w2i w) (dimindex (:'a))
+Proof
+  rw [ifits_def, GSYM INT_MIN_def] >>
+  metis_tac [INT_MIN, w2i_ge, integer_wordTheory.INT_MAX_def, w2i_le,
+             intLib.COOPER_PROVE ``!(x:int) y. x ≤ y - 1 ⇔ x < y``]
+QED
+
+Theorem truncate_2comp_fits:
+  ∀i size. 0 < size ⇒ ifits (truncate_2comp i size) size
+Proof
+  rw [truncate_2comp_def, ifits_def] >>
+  qmatch_goalsub_abbrev_tac `(i + s1) % s2` >>
+  `s2 ≠ 0 ∧ ¬(s2 < 0)` by rw [Abbr `s2`]
+  >- (
+    `0 ≤ (i + s1) % s2` suffices_by intLib.COOPER_TAC >>
+    drule INT_MOD_BOUNDS >>
+    rw [])
+  >- (
+    `(i + s1) % s2 < 2 * s1` suffices_by intLib.COOPER_TAC >>
+    `2 * s1 = s2` by rw [Abbr `s1`, Abbr `s2`, GSYM EXP] >>
+    drule INT_MOD_BOUNDS >>
+    rw [Abbr `s1`, Abbr `s2`])
+QED
+
+Theorem fits_ident:
+  ∀i size. 0 < size ⇒ (ifits i size ⇔ truncate_2comp i size = i)
+Proof
+  rw [ifits_def, truncate_2comp_def] >>
+  rw [intLib.COOPER_PROVE ``!(x:int) y z. x - y = z <=> x = y + z``] >>
+  qmatch_goalsub_abbrev_tac `(_ + s1) % s2` >>
+  `s2 ≠ 0 ∧ ¬(s2 < 0)` by rw [Abbr `s2`] >>
+  `2 * s1 = s2` by rw [Abbr `s1`, Abbr `s2`, GSYM EXP] >>
+  eq_tac >>
+  rw []
+  >- (
+    simp [Once INT_ADD_COMM] >>
+    irule INT_LESS_MOD >>
+    rw [] >>
+    intLib.COOPER_TAC)
+  >- (
+   `0 ≤ (i + s1) % (2 * s1)` suffices_by intLib.COOPER_TAC >>
+    drule INT_MOD_BOUNDS >>
+    simp [])
+  >- (
+   `(i + s1) % (2 * s1) < 2 * s1` suffices_by intLib.COOPER_TAC >>
+    drule INT_MOD_BOUNDS >>
+    simp [])
+QED
+
+Theorem i2n_n2i:
+  !n size. 0 < size ⇒ (nfits n size ⇔ (i2n (n2i n size) = n))
+Proof
+  rw [nfits_def, n2i_def, i2n_def] >> rw []
+  >- intLib.COOPER_TAC
+  >- (
+    `2 ** size ≤ n` by intLib.COOPER_TAC >> simp [INT_SUB] >>
+    Cases_on `n = 0` >> fs [] >>
+    `n - 2 ** size < n` suffices_by intLib.COOPER_TAC >>
+    irule SUB_LESS >> simp [])
+  >- (
+    `2 ** (size - 1) < 2 ** size` suffices_by intLib.COOPER_TAC >>
+    fs [])
+QED
+
+Theorem n2i_i2n:
+  !i size. 0 < size ⇒ (ifits i size ⇔ (n2i (i2n (IntV i size)) size) = IntV i size)
+Proof
+  rw [ifits_def, n2i_def, i2n_def] >> rw [] >> fs []
+  >- (
+    eq_tac >> rw []
+    >- (
+      simp [intLib.COOPER_PROVE ``∀(x:int) y z. x - y = z ⇔ x = y + z``] >>
+      `2 ** (size - 1) < 2 ** size` suffices_by intLib.COOPER_TAC >>
+      fs [INT_OF_NUM])
+    >- (
+      fs [intLib.COOPER_PROVE ``∀(x:int) y z. x - y = z ⇔ x = y + z``] >>
+      fs [INT_OF_NUM] >>
+      `?j. i = -j` by intLib.COOPER_TAC >> rw [] >> fs [] >>
+      qpat_x_assum `_ ≤ Num _` mp_tac >>
+      fs [GSYM INT_OF_NUM] >>
+      ASM_REWRITE_TAC [GSYM INT_LE] >> rw [] >>
+      `2 ** size = 2 * 2 ** (size - 1)` by rw [GSYM EXP, ADD1] >> fs [] >>
+      intLib.COOPER_TAC)
+    >- intLib.COOPER_TAC)
+  >- (
+    eq_tac >> rw []
+    >- intLib.COOPER_TAC
+    >- intLib.COOPER_TAC >>
+    `0 ≤ i` by intLib.COOPER_TAC >>
+    fs [GSYM INT_OF_NUM] >>
+    `&(2 ** size) = 0` by intLib.COOPER_TAC >>
+    fs [])
+  >- (
+    eq_tac >> rw []
+    >- (
+      `2 ** size = 2 * 2 ** (size - 1)` by rw [GSYM EXP, ADD1] >> fs [] >>
+      intLib.COOPER_TAC)
+    >- intLib.COOPER_TAC
+    >- intLib.COOPER_TAC)
+  >- intLib.COOPER_TAC
+QED
+
+Theorem w2n_i2n:
+  ∀w. w2n (w : 'a word) = i2n (IntV (w2i w) (dimindex (:'a)))
+Proof
+  rw [i2n_def] >> Cases_on `w` >> fs []
+  >- (
+    `INT_MIN (:α) ≤ n`
+    by (
+      fs [w2i_def] >> rw [] >>
+      BasicProvers.EVERY_CASE_TAC >> fs [word_msb_n2w_numeric] >>
+      rfs []) >>
+    rw [w2i_n2w_neg, dimword_def, int_arithTheory.INT_NUM_SUB])
+  >- (
+    `n < INT_MIN (:'a)`
+    by (
+      fs [w2i_def] >> rw [] >>
+      BasicProvers.EVERY_CASE_TAC >> fs [word_msb_n2w_numeric] >>
+      rfs []) >>
+    rw [w2i_n2w_pos])
+QED
+
+export_theory ();
